@prefix : <http://www.semanticweb.org/sanar/ontologies/2024/6/untitled-ontology-507/> .
@prefix owl: <http://www.w3.org/2002/07/owl#> .
@prefix rdf: <http://www.w3.org/1999/02/22-rdf-syntax-ns#> .
@prefix xml: <http://www.w3.org/XML/1998/namespace> .
@prefix xsd: <http://www.w3.org/2001/XMLSchema#> .
@prefix rdfs: <http://www.w3.org/2000/01/rdf-schema#> .
@base <http://www.semanticweb.org/sanar/ontologies/2024/6/untitled-ontology-507/> .

<http://www.semanticweb.org/MMKGDataspaces/ontology/2024/1/Dataspaces> rdf:type owl:Ontology ;
                                                                        owl:imports <http://purl.org/dc/elements/1.1/> ,
                                                                                    <http://www.semanticweb.org/MM/ontology/2023/1/mm> ,
                                                                                    <http://www.w3.org/2006/time#2016> ;
                                                                        rdfs:comment "This file contains the alignment of the multi-modal ODP with the Ontology for Multimodal Knowledge Graphs for Data Spaces. Since, we could not find any link pointing to the source file of the ontology, we did the alignment by creating a new file and importing the TBox of the multi-modal ODP." .

#################################################################
#    Annotation properties
#################################################################

###  http://purl.org/dc/terms/created
<http://purl.org/dc/terms/created> rdfs:domain :Source .


###  http://purl.org/dc/terms/identifier
<http://purl.org/dc/terms/identifier> rdf:type owl:AnnotationProperty ;
                                      rdfs:domain :Scene .


###  http://purl.org/dc/terms/title
<http://purl.org/dc/terms/title> rdfs:domain :Source .


#################################################################
#    Classes
#################################################################

###  http://www.semanticweb.org/sanar/ontologies/2024/6/untitled-ontology-507/Scene
:Scene rdf:type owl:Class ;
       rdfs:subClassOf <http://www.semanticweb.org/MM/ontology/2023/1/mm#Multi-ModalEntity> ;
       rdfs:comment "Concecpt used in the Ontology for Multimodal Knowledge Graphs for Data Spaces to represent a scene captured by a camera." ;
       rdfs:label "Scena"@it ,
                  "Scene"@en .


###  http://www.semanticweb.org/sanar/ontologies/2024/6/untitled-ontology-507/Source
:Source rdf:type owl:Class ;
        rdfs:subClassOf <http://www.semanticweb.org/MM/ontology/2023/1/mm#ModalDescriptor> ;
        rdfs:comment "Concecpt used in the Ontology for Multimodal Knowledge Graphs for Data Spaces to represent  unstructured data files received from the camera, such as image." ;
        rdfs:label "Sorgente"@it ,
                   "Source"@en .


###  Generated by the OWL API (version 4.5.25.2023-02-15T19:15:49Z) https://github.com/owlcs/owlapi
